src/Main.lean
@@ -1,17 +1,12 @@
 import LeanEVM.State
+import LeanEVM.Instructions.Arithmetic
 
-/- =============================================================== -/
-/- Main -/
-/- =============================================================== -/
+def even (k : Nat) : Prop :=
+  (k % 2) = 0
 
-def main : IO Unit :=
-  IO.println "Hello world"
-
-
-abbrev byte2 := Fin 256
-
-def test(n:List byte2) := n.length
-
-example : (test [1,2]) = 2 :=
+def test (k:Nat)(p:even k) : even (k+2) :=
 by
-  simp_arith
+  unfold even
+  have q : (k+2) % 2 = k % 2 := Nat.add_mod_right k 2
+  rw [q]
+  exact p
